Tealeaves/Examples/STLC/Simplification.v
@@ -19,13 +19,13 @@ Proof.
   intros. simplify_LN. reflexivity.
 Qed.
 
-Theorem term_lcn2 : forall (X : typ) (t : term LN) (m : nat),
+Theorem term_lcn2 : forall (X : typ) (t : term) (m : nat),
     LCn m (lam X t) <-> LCn (S m) t.
 Proof.
   intros. simplify_LN. reflexivity.
 Qed.
 
-Theorem term_lcn3 : forall (t1 t2 : term LN) (m : nat),
+Theorem term_lcn3 : forall (t1 t2 : term) (m : nat),
     LCn m (⟨t1⟩(t2)) <->
       LCn m t1 /\ LCn m t2.
 Proof.
@@ -44,13 +44,13 @@ Proof.
   intros. simplify_LN. reflexivity.
 Qed.
 
-Theorem term_lc2 : forall (X : typ) (t : term LN),
+Theorem term_lc2 : forall (X : typ) (t : term),
     LC (lam X t) <-> LCn 1 t.
 Proof.
   intros. simplify_LN. reflexivity.
 Qed.
 
-Theorem term_lc3 : forall (t1 t2 : term LN),
+Theorem term_lc3 : forall (t1 t2 : term),
     LC (⟨t1⟩ (t2)) <-> LC t1 /\ LC t2.
 Proof.
   intros. simplify_LN. reflexivity.
@@ -69,13 +69,13 @@ Section term_container_rewrite.
     intros. simplify. reflexivity.
   Qed.
 
-  Lemma tolist_term_rw2: forall (X: typ) (t: term A),
+  Lemma tolist_term_rw2: forall (X: typ) (t: term),
       tolist (lam X t) = tolist t.
   Proof.
     intros. simplify. reflexivity.
   Qed.
 
-  Lemma tolist_term_rw3: forall (t1 t2: term A),
+  Lemma tolist_term_rw3: forall (t1 t2: term),
       tolist (app t1 t2) = tolist t1 ++ tolist t2.
   Proof.
     intros. simplify. reflexivity.
@@ -86,13 +86,13 @@ Section term_container_rewrite.
     intros. simplify. reflexivity.
   Qed.
 
-  Lemma toset_term_rw2: forall (X: typ) (t: term A),
+  Lemma toset_term_rw2: forall (X: typ) (t: term),
       tosubset (lam X t) = tosubset t.
   Proof.
     intros. simplify_tosubset. reflexivity.
   Qed.
 
-  Lemma toset_term_rw3: forall (t1 t2: term A),
+  Lemma toset_term_rw3: forall (t1 t2: term),
       tosubset (app t1 t2) = tosubset t1 ∪ tosubset t2.
   Proof.
     intros. simplify. reflexivity.
@@ -104,13 +104,13 @@ Section term_container_rewrite.
     intros. simplify. reflexivity.
   Qed.
 
-  Lemma in_term_rw2: forall (y: A) (X: typ) (t: term A),
+  Lemma in_term_rw2: forall (y: A) (X: typ) (t: Lam A),
       y ∈ (lam X t) <-> y ∈ t.
   Proof.
     intros. simplify. reflexivity.
   Qed.
 
-  Lemma in_term_3: forall (t1 t2: term A) (y: A),
+  Lemma in_term_3: forall (t1 t2: Lam A) (y: A),
       y ∈ (app t1 t2) <-> y ∈ t1 \/ y ∈ t2.
   Proof.
     intros. simplify. reflexivity.
@@ -121,8 +121,6 @@ End term_container_rewrite.
 (** ** Rewriting lemmas for <<free>>, <<freeset>> *)
 (******************************************************************************)
 Section term_free_rewrite.
-
-  Variable (A : Type).
 
   Definition term_free11 : forall (b : nat),
       free (tvar (Bd b)) = [].
@@ -148,25 +146,25 @@ Section term_free_rewrite.
     intros. simplify. reflexivity.
   Qed.
 
-  Definition term_free2 : forall (t : term LN) (X : typ),
+  Definition term_free2 : forall (t : term) (X : typ),
       free (lam X t) = free t.
   Proof.
     intros. simplify_LN. reflexivity.
   Qed.
 
-  Definition term_in_free2 : forall (x : atom) (t : term LN) (X : typ),
+  Definition term_in_free2 : forall (x : atom) (t : term) (X : typ),
       x ∈ free (lam X t) <-> x ∈ free t.
   Proof.
     intros. simplify. reflexivity.
   Qed.
 
-  Definition term_free3 : forall (x : atom) (t1 t2 : term LN),
+  Definition term_free3 : forall (x : atom) (t1 t2 : term),
       free (app t1 t2) = free t1 ++ free t2.
   Proof.
     intros. simplify. reflexivity.
   Qed.
 
-  Definition term_in_free3 : forall (x : atom) (t1 t2 : term LN),
+  Definition term_in_free3 : forall (x : atom) (t1 t2 : term),
       x ∈ free (app t1 t2) <-> x ∈ free t1 \/ x ∈ free t2.
   Proof.
     intros. simplify. reflexivity.
@@ -184,13 +182,13 @@ Section term_free_rewrite.
     intros. simplify_FV. reflexivity.
   Qed.
 
-  Lemma term_in_FV2 : forall (x : atom) (t : term LN) (X : typ),
+  Lemma term_in_FV2 : forall (x : atom) (t : term) (X : typ),
       AtomSet.In x (FV (lam X t)) <-> AtomSet.In x (FV t).
   Proof.
     intros. simplify_FV. reflexivity.
   Qed.
 
-  Lemma term_in_FV3 : forall (x : atom) (t1 t2 : term LN),
+  Lemma term_in_FV3 : forall (x : atom) (t1 t2 : term),
       AtomSet.In x (FV (app t1 t2)) <->
         AtomSet.In x (FV t1) \/ AtomSet.In x (FV t2).
   Proof.
@@ -211,13 +209,13 @@ Section term_free_rewrite.
     intros. simplify_FV. fsetdec.
   Qed.
 
-  Lemma term_FV2 : forall (t : term LN) (X : typ),
+  Lemma term_FV2 : forall (t : term) (X : typ),
       FV (lam X t) [=] FV t.
   Proof.
     intros. simplify_FV. fsetdec.
   Qed.
 
-  Lemma term_FV3 : forall (t1 t2 : term LN),
+  Lemma term_FV3 : forall (t1 t2 : term),
       FV (app t1 t2) [=] FV t1 ∪ FV t2.
   Proof.
     intros. simplify_FV. fsetdec.
@@ -237,13 +235,13 @@ Section term_foldMapd_rewrite.
     intros. simplify_foldMapd. reflexivity.
   Qed.
 
-  Lemma term_foldMapd2 : forall X (t : term A),
+  Lemma term_foldMapd2 : forall X (t : Lam A),
       foldMapd f (λ X t) = foldMapd (f ⦿ 1) t.
   Proof.
     intros. simplify_foldMapd. reflexivity.
   Qed.
 
-  Lemma term_foldMapd3 : forall (t1 t2 : term A),
+  Lemma term_foldMapd3 : forall (t1 t2 : Lam A),
       foldMapd f (⟨t1⟩ (t2)) = foldMapd f t1 ● foldMapd f t2.
   Proof.
     intros. simplify_foldMapd. reflexivity.
@@ -261,13 +259,13 @@ Section term_ind_rewrite.
     intros. simplify. reflexivity.
   Qed.
 
-  Lemma term_ind2 : forall (t : term LN) (l : LN) (n : nat) (X : typ),
+  Lemma term_ind2 : forall (t : term) (l : LN) (n : nat) (X : typ),
       (n, l) ∈d t = (S n, l) ∈d (λ X t).
   Proof.
     intros. simplify_element_ctx_of. reflexivity.
   Qed.
 
-  Lemma term_ind2_nZ : forall (t : term LN) (l : LN) (n : nat) (X : typ),
+  Lemma term_ind2_nZ : forall (t : term) (l : LN) (n : nat) (X : typ),
       (n, l) ∈d (λ X t) -> n <> 0.
   Proof.
     introv.
@@ -279,7 +277,8 @@ Section term_ind_rewrite.
       easy.
   Qed.
 
-  Lemma term_ind3 : forall (t1 t2 : term LN) (n : nat) (l : LN),
+  (* TODO: This is a good example for improving simplify execution times. *)
+  Lemma term_ind3 : forall (t1 t2 : term) (n : nat) (l : LN),
       (n, l) ∈d (⟨t1⟩ (t2)) <-> (n, l) ∈d t1 \/ (n, l) ∈d t2.
   Proof.
     intros. simplify. reflexivity.
@@ -289,13 +288,13 @@ End term_ind_rewrite.
 
 (** ** Rewriting lemmas for <<open>> *)
 (******************************************************************************)
-Lemma open_term_rw2: forall (t1 t2: term LN) u,
+Lemma open_term_rw2: forall (t1 t2: term) u,
     open u (app t1 t2) = app (open u t1) (open u t2).
 Proof.
   intros. simplify_open. reflexivity.
 Qed.
 
-Lemma open_term_rw3: forall τ (t: term LN) u,
+Lemma open_term_rw3: forall τ (t: term) u,
     open u (λ τ t) = λ τ (bindd (open_loc u ⦿ 1) t).
 Proof.
   intros. simplify_open. reflexivity.
@@ -303,14 +302,14 @@ Qed.
 
 (** ** Rewriting lemmas for <<subst>> *)
 (******************************************************************************)
-Lemma subst_term_rw2: forall (t1 t2: term LN) x u,
+Lemma subst_term_rw2: forall (t1 t2: term) x u,
     subst x u (app t1 t2) =
       app (subst x u t1) (subst x u t2).
 Proof.
   intros. simplify_subst. reflexivity.
 Qed.
 
-Lemma subst_term_rw3: forall τ (t: term LN) x u,
+Lemma subst_term_rw3: forall τ (t: term) x u,
     subst x u (λ τ t) =
       λ τ (subst x u t).
 Proof.
